src/VmSemantics.v
@@ -68,6 +68,7 @@ Proof.
     destruct r.
     destruct a;
       simpl;
+      df;
       repeat rewrite app_assoc;
       reflexivity.
   -
@@ -427,6 +428,18 @@ Ltac do_restl :=
       ltac:(eapply restl; [apply H2 | apply H])
   end.
 
+Check splitEv_l.
+
+Lemma splitEv_T_l_LEFT: forall e bits bits' es e0,
+    et_size e = es ->
+    splitEv_l LEFT (evc bits e) = (evc bits' e0) ->
+    et_size e0 = es. (* (splitEv_T_l LEFT es). *)
+Proof.
+  intros.
+  ff.
+Defined.
+
+(*
 Lemma splitEv_T_l_LEFT: forall e es e0,
     Ev_Shape e es ->
     splitEv_l LEFT e = e0 ->
@@ -441,13 +454,53 @@ Defined.
 Axiom remote_Ev_Shape: forall e es t n,
     Ev_Shape e es ->
     Ev_Shape (toRemote t n e) (eval (unanno t) n es).
+ *)
 
-Lemma cvm_refines_lts_evidence : forall t tr tr' e e' p p' es e's,
+Check length.
+
+Definition Ev_Shape' (bits:list BS) (et:Evidence) :=
+  length bits = et_size et.
+
+Axiom remote_Ev_Shape: forall et et' t n bits bits',
+    Ev_Shape' bits et ->
+    toRemote t n (evc bits et) = evc bits' et' ->
+    Ev_Shape' bits' (eval (unanno t) n et).
+
+Lemma cvm_refines_lts_evidence : forall t tr tr' bits bits' et et' p p',
     well_formed_r t ->
-    copland_compile t (mk_st e tr p) = (Some tt, (mk_st e' tr' p')) ->
-    Ev_Shape e es ->
-    Term_Defs.eval (unanno t) p es = e's ->
-    Ev_Shape e' e's.
+    copland_compile t (mk_st (evc bits et) tr p) = (Some tt, (mk_st (evc bits' et') tr' p')) ->
+    (*Ev_Shape' bits et -> *)
+    (*
+    Term_Defs.eval (unanno t) p es = e's -> *)
+    et' = (Term_Defs.eval (unanno t) p et). (* /\
+    Ev_Shape' bits' et'. *)
+
+Proof.
+Admitted.
+
+Lemma cvm_evidence_size : forall t tr tr' bits bits' et et' p p',
+    well_formed_r t ->
+    copland_compile t (mk_st (evc bits et) tr p) = (Some tt, (mk_st (evc bits' et') tr' p')) ->
+    Ev_Shape' bits et ->
+    (*
+    Term_Defs.eval (unanno t) p es = e's -> *)
+    (*et' = (Term_Defs.eval (unanno t) p et) /\ *)
+    Ev_Shape' bits' (Term_Defs.eval (unanno t) p et).
+
+Proof.
+Admitted.
+
+
+(*
+Lemma cvm_refines_lts_evidence : forall t tr tr' bits bits' et et' p p',
+    well_formed_r t ->
+    copland_compile t (mk_st (evc bits et) tr p) = (Some tt, (mk_st (evc bits' et') tr' p')) ->
+    Ev_Shape' bits et ->
+    (*
+    Term_Defs.eval (unanno t) p es = e's -> *)
+    et' = (Term_Defs.eval (unanno t) p et) /\
+    Ev_Shape' bits' et'.
+
 Proof.
   induction t; intros.
   -
@@ -455,8 +508,221 @@ Proof.
       try (
           df;
           eauto).
+    +
+      split.
+      eauto.
+      unfold Ev_Shape' in *.
+      ff.
+    +
+      split.
+      eauto.
+      unfold Ev_Shape' in *.
+      ff.
+
+    +
+      split.
+      eauto.
+      unfold Ev_Shape' in *.
+      ff.
+
+  -
+    repeat df. 
+    annogo.
+    do_wf_pieces.
+    edestruct IHt; eauto.
+    rewrite <- H3.
+    apply copland_compile_at.
+    eauto.
+
+  -
+    do_wf_pieces.
+    do_suffix blah.
+    destruct_conjs.
+    subst.
+
+    edestruct alseq_decomp.
+    eassumption.
+    eapply restl.
+    eassumption.
+    eassumption.
+    destruct_conjs.
+    df.
+    dosome.
+
+    destruct x.
+    vmsts.
+
+    edestruct IHt1.
+    eassumption.
+    eassumption.
+    eassumption.
+    subst.
+
+    edestruct IHt2.
+    eassumption. eassumption.
+    eassumption.
+    subst.
+    split.
+    repeat do_pl_immut.
+    subst.
+    eauto.
+    eassumption.     
+  -
+    do_wf_pieces.
+    df.
+    repeat break_match;
+      try solve_by_inversion;
+      try (df; tauto).
+    +
+      df.
+      annogo.
+      simpl in *.
+      do_suffix blah.
+      do_suffix blah'.
+      destruct_conjs; subst.
+      repeat do_restl.
+
+      
+      destruct s; ff.
+      ++
+        edestruct IHt1; eauto.
+        subst.
+        edestruct IHt2.
+        eassumption.
+        eassumption.
+        unfold Ev_Shape'. ff.
+        subst.
+        repeat do_pl_immut. subst.
+        split. eauto. df.
+        unfold Ev_Shape' in *.
+        ff.
+        Search length.
+        rewrite app_length.
+        subst.
+        lia.
+      ++
+        edestruct IHt1; eauto. cbv. lia.
+        subst.
+        edestruct IHt2; eauto.
+        unfold Ev_Shape'. ff.
+        subst.
+        repeat do_pl_immut. subst.
+        split. eauto. df.
+        unfold Ev_Shape' in *.
+        ff.
+        Search length.
+        rewrite app_length.
+        subst.
+        lia.
+      ++
+        edestruct IHt1; eauto.
+        subst.
+        edestruct IHt2; eauto.
+        unfold Ev_Shape'. ff.
+        subst.
+        repeat do_pl_immut. subst.
+        split. eauto. df.
+        unfold Ev_Shape' in *.
+        ff.
+        Search length.
+        rewrite app_length.
+        subst.
+        lia.
+  -
+    do_wf_pieces.
+    df.
+    repeat break_match;
+      try solve_by_inversion;
+      try (df; tauto).
+    +
+      df.
+      annogo.
+      simpl in *.
+      do_suffix blah.
+      do_suffix blah'.
+      destruct_conjs; subst.
+      repeat do_restl.
+
+      
+      destruct s; ff.
+      ++
+        edestruct IHt1; eauto.
+        subst.
+        edestruct IHt2.
+        eassumption.
+        eassumption.
+        unfold Ev_Shape'. ff.
+        subst.
+        repeat do_pl_immut. subst.
+        split. eauto. df.
+        unfold Ev_Shape' in *.
+        ff.
+        Search length.
+        rewrite app_length.
+        subst.
+        lia.
+      ++
+        edestruct IHt1; eauto. cbv. lia.
+        subst.
+        edestruct IHt2; eauto.
+        unfold Ev_Shape'. ff.
+        subst.
+        repeat do_pl_immut. subst.
+        split. eauto. df.
+        unfold Ev_Shape' in *.
+        ff.
+        Search length.
+        rewrite app_length.
+        subst.
+        lia.
+      ++
+        edestruct IHt1; eauto.
+        subst.
+        edestruct IHt2; eauto.
+        unfold Ev_Shape'. ff.
+        subst.
+        repeat do_pl_immut. subst.
+        split. eauto. df.
+        unfold Ev_Shape' in *.
+        ff.
+        Search length.
+        rewrite app_length.
+        subst.
+        lia.
+Defined.
+*)
+
+(*
+Proof.
+  induction t; intros.
+  -
+    destruct a;
+      try (
+          df;
+          eauto).
+    +
+      split.
+      eauto.
+      unfold Ev_Shape' in *.
+      ff.
+    +
+      split.
+      eauto.
+      unfold Ev_Shape' in *.
+      ff.
+
+    +
+      split.
+      eauto.
+      unfold Ev_Shape' in *.
+      ff.
+
+
+
 
     
+
+  (*  
     +
       assert (Ev_Shape e (et_fun e)).
       {
@@ -471,6 +737,7 @@ Proof.
       }
       subst.
       eauto.
+*)
       
       
       
@@ -597,6 +864,11 @@ Proof.
           ff.
           eauto.
 Defined.
+*)
+
+
+
+
 
 Axiom remote_LTS: forall t n et, 
     lstar (conf t n et) (remote_events t n) (stop n (aeval t n et)).
@@ -625,6 +897,7 @@ Proof.
     eauto. 
 Defined.
 
+(*
 Lemma evshape_split_l: forall e et s,
     Ev_Shape e et ->
     Ev_Shape ((splitEv_l s e)) (splitEv_T_l s et).
@@ -644,7 +917,467 @@ Proof.
   induction e; intros;
     try (destruct s; ff; tauto).
 Defined.
-   
+ *)
+
+Lemma cvm_refines_lts_event_ordering : forall t tr bits bits' et et' p p',
+    well_formed_r t ->
+    (*Ev_Shape e et -> *)
+    copland_compile t (mk_st (evc bits et) [] p) = (Some tt, (mk_st (evc bits' et') tr p')) ->
+    lstar (conf t p et) tr (stop p (aeval t p et)).
+Proof.
+  intros t tr bits bits' et et' p p' H H'.
+  generalizeEverythingElse t.
+  induction t; intros.
+  - (* aasp case *)
+    destruct a;
+      df;
+      econstructor; try (econstructor; reflexivity).
+
+    (*
+    
+    +
+      assert (et = et_fun e).
+      {
+        eapply evshape_determ; eauto.
+        apply ev_evshape; eauto.
+      }
+      rewrite <- H0.
+      econstructor; try (econstructor; reflexivity). *)
+      
+      
+  - (* aatt case *)
+    destruct r.
+    repeat (df; try dohtac; df).
+    
+    assert (lstar (conf t n et) (remote_events t n) (stop n (aeval t n et))).
+    {
+      apply remote_LTS.
+    }
+
+    
+
+    (*
+    pose ev_evshape.
+    pose (e0 e).
+    
+    assert (et_fun e = et).
+    {
+      pose ev_evshape.
+      pose (e0 e).
+      eapply evshape_determ.
+      eassumption.
+      eassumption.
+    }
+    rewrite H1. *)
+    
+
+    eapply lstar_tran.
+    econstructor.
+    simpl.
+    eapply lstar_transitive.
+    eapply lstar_strem.
+    cbn.
+    
+    apply H0.
+
+    econstructor.
+    apply stattstop.
+    econstructor.
+  -  
+    do_wf_pieces.
+    edestruct alseq_decomp; eauto.
+    destruct_conjs.
+    destruct x.
+    econstructor.
+    econstructor.
+    subst.
+    eapply lstar_transitive.
+    eapply lstar_stls.
+    df.
+    eapply IHt1.
+    eassumption.
+    eassumption.
+
+    eapply lstar_silent_tran.
+    apply stlseqstop.
+    df.
+    repeat do_pl_immut.
+    subst.   
+    eapply IHt2. (*with (e:= x). *)
+    eassumption.
+    Check eval.
+    assert (e0 = Term_Defs.eval (unanno t1) p et).
+    eapply cvm_refines_lts_evidence; eauto.
+
+    subst.
+    rewrite <- eval_aeval.
+    
+    apply H6.
+    
+  -    
+    do_wf_pieces.
+    destruct r; destruct s.
+    +
+    df.
+    vmsts.
+    dosome.
+    df.
+
+    do_suffix blah.
+    do_suffix blah'.
+    destruct_conjs; subst.
+    repeat do_restl.
+    
+    repeat do_pl_immut.
+    subst.
+    repeat rewrite <- app_assoc.
+
+    eapply lstar_tran.
+    econstructor.
+    simpl.
+
+    eapply lstar_transitive.
+    simpl.
+
+    eapply lstar_stbsl.  
+     
+    eapply IHt1.
+    eassumption.
+    (*
+    2: {
+      eassumption.
+    } *)
+    eassumption.
+  
+    unfold run_cvm in *.
+    monad_unfold.
+
+    eapply lstar_silent_tran.
+    apply stbslstop.
+    
+    eapply lstar_transitive.
+    eapply lstar_stbsr.
+        
+    eapply IHt2.
+    eassumption.
+    (*
+    2: {
+      eassumption.
+      } *)
+    eassumption.
+
+    Print step.
+    
+    
+    econstructor.
+
+    eapply stbsrstop.
+    econstructor.
+    +
+      
+    df.
+    vmsts.
+    dosome.
+    df.
+
+    do_suffix blah.
+    do_suffix blah'.
+    destruct_conjs; subst.
+    repeat do_restl.
+    
+    repeat do_pl_immut.
+    subst.
+    repeat rewrite <- app_assoc.
+
+    eapply lstar_tran.
+    econstructor.
+    simpl.
+
+    eapply lstar_transitive.
+    simpl.
+
+    eapply lstar_stbsl.  
+     
+    eapply IHt1.
+    eassumption.
+    (*
+    2: {
+      eassumption.
+    } *)
+    eassumption.
+  
+    unfold run_cvm in *.
+    monad_unfold.
+
+    eapply lstar_silent_tran.
+    apply stbslstop.
+    
+    eapply lstar_transitive.
+    eapply lstar_stbsr.
+        
+    eapply IHt2.
+    eassumption.
+    (*
+    2: {
+      eassumption.
+      } *)
+    eassumption.
+
+    Print step.
+    
+    
+    econstructor.
+
+    eapply stbsrstop.
+    econstructor.
+    +
+      df.
+    vmsts.
+    dosome.
+    df.
+
+    do_suffix blah.
+    do_suffix blah'.
+    destruct_conjs; subst.
+    repeat do_restl.
+    
+    repeat do_pl_immut.
+    subst.
+    repeat rewrite <- app_assoc.
+
+    eapply lstar_tran.
+    econstructor.
+    simpl.
+
+    eapply lstar_transitive.
+    simpl.
+
+    eapply lstar_stbsl.  
+     
+    eapply IHt1.
+    eassumption.
+    (*
+    2: {
+      eassumption.
+    } *)
+    eassumption.
+  
+    unfold run_cvm in *.
+    monad_unfold.
+
+    eapply lstar_silent_tran.
+    apply stbslstop.
+    
+    eapply lstar_transitive.
+    eapply lstar_stbsr.
+        
+    eapply IHt2.
+    eassumption.
+    (*
+    2: {
+      eassumption.
+      } *)
+    eassumption.
+
+    Print step.
+    
+    
+    econstructor.
+
+    eapply stbsrstop.
+    econstructor.
+
+  -    
+    do_wf_pieces.
+    destruct r; destruct s.
+    +
+    df.
+    vmsts.
+    dosome.
+    df.
+
+    do_suffix blah.
+    do_suffix blah'.
+    destruct_conjs; subst.
+    repeat do_restl.
+    
+    repeat do_pl_immut.
+    subst.
+    repeat rewrite <- app_assoc.
+
+    eapply lstar_tran.
+    econstructor.
+    simpl.
+
+    eapply lstar_transitive.
+    simpl.
+    Locate lstar_stbparl.
+
+    eapply lstar_stbparl.  
+     
+    eapply IHt1.
+    eassumption.
+    (*
+    2: {
+      eassumption.
+    } *)
+    eassumption.
+  
+    unfold run_cvm in *.
+    monad_unfold.
+
+    (*
+    eapply lstar_transitive.
+    
+    apply stbpstepleft.
+    apply stbpstop. *)
+    
+    eapply lstar_transitive.
+    eapply lstar_stbparr.
+        
+    eapply IHt2.
+    eassumption.
+    (*
+    2: {
+      eassumption.
+      } *)
+    eassumption.
+
+    Print step.
+    
+    
+    econstructor.
+
+    eapply stbpstop.
+    econstructor.
+        +
+    df.
+    vmsts.
+    dosome.
+    df.
+
+    do_suffix blah.
+    do_suffix blah'.
+    destruct_conjs; subst.
+    repeat do_restl.
+    
+    repeat do_pl_immut.
+    subst.
+    repeat rewrite <- app_assoc.
+
+    eapply lstar_tran.
+    econstructor.
+    simpl.
+
+    eapply lstar_transitive.
+    simpl.
+    Locate lstar_stbparl.
+
+    eapply lstar_stbparl.  
+     
+    eapply IHt1.
+    eassumption.
+    (*
+    2: {
+      eassumption.
+    } *)
+    eassumption.
+  
+    unfold run_cvm in *.
+    monad_unfold.
+
+    (*
+    eapply lstar_transitive.
+    
+    apply stbpstepleft.
+    apply stbpstop. *)
+    
+    eapply lstar_transitive.
+    eapply lstar_stbparr.
+        
+    eapply IHt2.
+    eassumption.
+    (*
+    2: {
+      eassumption.
+      } *)
+    eassumption.
+
+    Print step.
+    
+    
+    econstructor.
+
+    eapply stbpstop.
+    econstructor.
+
+        +
+    df.
+    vmsts.
+    dosome.
+    df.
+
+    do_suffix blah.
+    do_suffix blah'.
+    destruct_conjs; subst.
+    repeat do_restl.
+    
+    repeat do_pl_immut.
+    subst.
+    repeat rewrite <- app_assoc.
+
+    eapply lstar_tran.
+    econstructor.
+    simpl.
+
+    eapply lstar_transitive.
+    simpl.
+    Locate lstar_stbparl.
+
+    eapply lstar_stbparl.  
+     
+    eapply IHt1.
+    eassumption.
+    (*
+    2: {
+      eassumption.
+    } *)
+    eassumption.
+  
+    unfold run_cvm in *.
+    monad_unfold.
+
+    (*
+    eapply lstar_transitive.
+    
+    apply stbpstepleft.
+    apply stbpstop. *)
+    
+    eapply lstar_transitive.
+    eapply lstar_stbparr.
+        
+    eapply IHt2.
+    eassumption.
+    (*
+    2: {
+      eassumption.
+      } *)
+    eassumption.
+
+    Print step.
+    
+    
+    econstructor.
+
+    eapply stbpstop.
+    econstructor.
+Defined.
+
+
+
+
+
+(*
 Lemma cvm_refines_lts_event_ordering : forall t tr e e' et p p',
     well_formed_r t ->
     Ev_Shape e et ->
@@ -1056,21 +1789,22 @@ Proof.
 
     econstructor.
 Defined.
+*)
 
-Lemma cvm_refines_lts_event_ordering_corrolary : forall t tr et e e' p p',
+Lemma cvm_refines_lts_event_ordering_corrolary : forall t tr bits bits' et et' p p',
     well_formed_r t ->
-    Ev_Shape e et ->
-    copland_compile t (mk_st e [] p) = (Some tt, (mk_st e' tr p')) ->
+    (*Ev_Shape e et -> *)
+    copland_compile t (mk_st (evc bits et) [] p) = (Some tt, (mk_st (evc bits' et') tr p')) ->
     st_trace (run_cvm t
-                     (mk_st e [] p)) = tr ->
+                     (mk_st (evc bits et) [] p)) = tr ->
     lstar (conf t p et) tr (stop p (aeval t p et)).
 Proof.
   intros.
-  destruct (copland_compile t {| st_ev := e; st_trace := []; st_pl := p |}) eqn:hi.
+  destruct (copland_compile t {| st_ev := (evc bits et); st_trace := []; st_pl := p |}) eqn:hi.
   simpl in *.
   vmsts.
   simpl in *.
-  apply cvm_refines_lts_event_ordering with (t:=t) (tr:=tr) (e:=e) (p:=p) (e':=st_ev) (p':=st_pl); eauto.
+  apply cvm_refines_lts_event_ordering with (t:=t) (tr:=tr) (bits:=bits) (et:=et) (bits':=bits') (et':=et') (p:=p) (p':=st_pl); eauto.
   
   try dunit.
   rewrite hi.
@@ -1082,13 +1816,13 @@ Proof.
   solve_by_inversion.
 Defined.
 
-Theorem cvm_respects_event_system' : forall t tr ev0 ev1 e e' et,
+Theorem cvm_respects_event_system' : forall t tr ev0 ev1 bits bits' et et',
     well_formed_r t ->
-    Ev_Shape e et ->
+    (*Ev_Shape e et -> *)
     copland_compile 
       t
-      (mk_st e [] 0) =
-      (Some tt, (mk_st e' tr 0)) ->
+      (mk_st (evc bits et) [] 0) =
+      (Some tt, (mk_st (evc bits' et') tr 0)) ->
     prec (ev_sys t 0 et) ev0 ev1 ->
     earlier tr ev0 ev1.
 Proof.
@@ -1097,13 +1831,13 @@ Proof.
   eapply cvm_refines_lts_event_ordering; eauto.
 Defined.
 
-Theorem cvm_respects_event_system : forall t tr ev0 ev1 e e' t' et,
+Theorem cvm_respects_event_system : forall t tr ev0 ev1 bits bits' et et' t',
     t = annotated t' ->
-    Ev_Shape e et ->
+    (*Ev_Shape e et ->*)
     copland_compile
       t
-      (mk_st e [] 0) =
-    (Some tt, (mk_st e' tr 0)) ->
+      (mk_st (evc bits et) [] 0) =
+    (Some tt, (mk_st (evc bits' et') tr 0)) ->
     prec (ev_sys t 0 et) ev0 ev1 ->
     earlier tr ev0 ev1.
 Proof.
